KLR/NKI/TIR.lean
@@ -1,0 +1,168 @@
+/-
+Copyright (c) 2025 Amazon.com, Inc. or its affiliates. All Rights Reserved.
+Released under Apache 2.0 license as described in the file LICENSE.
+Authors: Paul Mure
+-/
+import KLR.NKI.Simplify
+import KLR.NKI.Types
+
+/-!
+# Typed IR for NKI
+
+This includes the following simplications
+- Tuples are removed
+- Function calls are curried and no default or keyword args are allowed
+- Binnary ops become calls of constant functions
+- `Stmt`s have `seq` which removed the need for `List Stmt`
+- Introduce let bindings in `Stmt`
+- No un-initialized variables allowed
+-/
+
+namespace KLR.NKI
+
+namespace TIR
+
+inductive Value where
+  | none
+  | bool (value : Bool)
+  | int (value : Int)
+  | float (value : Float)
+  | string (value : String)
+  | ellipsis
+  | tensor (shape : List Nat) (dtype : Core.Dtype)
+
+inductive Const where
+  -- logical
+  | land | lor
+  -- comparison
+  | eq | ne | lt | le | gt | ge
+  -- arithmetic
+  | add | sub | mul | div | mod | pow | floor
+  -- bitwise
+  | lshift | rshift | or | xor | and
+
+mutual
+
+inductive Index where
+  | coord (i : Expr)
+  | slice (l u step : Option Expr)
+
+structure Expr where
+  expr : Expr'
+  pos : Pos
+
+inductive Expr' where
+  | const (const : Const)
+  | value (value : Value)
+  | var (name : String)
+  | access (expr : Expr) (indices : List Index)
+  | ifExp (test body orelse : Expr)
+  | app (f : Expr) (arg : Expr)
+  | typApp (f : Expr) (arg : Expr)
+
+end
+
+mutual
+
+structure Stmt where
+  stmt : Stmt'
+  pos : Pos
+
+inductive Stmt' where
+  | expr (e : Expr)
+  | assert (e : Expr)
+  | ret (e : Expr)
+  | let_ (var : String) (ty : Types.Typ) (rhs : Expr)
+  | assign (lhs : Expr) (rhs : Expr)
+  | ifStm (e : Expr) (thn els : Stmt)
+  | forLoop (x : Expr) (iter : Expr) (body : Stmt)
+  | breakLoop
+  | continueLoop
+  | seq (s1 s2 : Stmt)
+
+end
+
+structure Fun where
+  name : String
+  file : String
+  line : Nat
+  body : Stmt
+  typArgs : List Types.Typ
+  args : List Types.Typ
+
+structure Kernel where
+  entry : String
+  typArgs : List Types.Typ
+  args : List Expr
+  funs : List Fun
+  globals : List Arg
+
+end TIR
+
+/-!
+# Lowering pass from basic NKI to TIR
+-/
+
+def Value.lower : Value → PosM TIR.Value
+  | none => return .none
+  | bool value => return .bool value
+  | int value => return .int value
+  | float value => return .float value
+  | string value => return .string value
+  | ellipsis => return .ellipsis
+  | tensor shape dtype =>
+    match Core.Dtype.fromString dtype with
+    | .some dtype => return .tensor shape dtype
+    | .none => throw s!"{dtype} is not a valid dtype"
+
+mutual
+
+def Expr.lowerOption : Option Expr → PosM (Option TIR.Expr)
+  | some e => return some (← e.lower)
+  | none => none
+
+def Index.lower : Index → PosM TIR.Index
+  | .coord i => return .coord (← i.lower)
+  | .slice l u step => do
+    let l ← Expr.lowerOption l
+    let u ← Expr.lowerOption u
+    let step ← Expr.lowerOption step
+    return .slice l u step
+
+def Expr.lower : Expr → PosM TIR.Expr
+  | { expr, pos } =>
+    withPos pos do
+      return {expr := ← expr.lower, pos := pos}
+
+def Expr'.lower : Expr' → PosM TIR.Expr'
+  | .value value => sorry
+  | .var name => sorry
+  | .proj expr name=> sorry
+  | .tuple elements => sorry
+  | .access expr indices => do
+    let expr ← expr.lower
+    let indices ← indices.mapM Index.lower
+    return .access expr indices
+  | .binOp op left right => sorry
+  | .ifExp test body orelse => sorry
+  | .call f args keywords => sorry
+
+end
+
+mutual
+
+def Stmt.lower : Stmt → PosM TIR.Stmt
+  | { stmt, pos } =>
+    withPos pos do
+      return {stmt := ← stmt.lower, pos := pos}
+
+def Stmt'.lower (stmt : Stmt') : PosM TIR.Stmt' :=
+  sorry
+
+end
+
+def Fun.lower (f : Fun) : PosM TIR.Fun :=
+  sorry
+
+def Kernel.lower (k : Kernel) : PosM TIR.Kernel :=
+  sorry
